Add solution for Pset2

pset2/Pset2.v
@@ -11,26 +11,31 @@ Require Import Frap Pset2Sig.
 Theorem either_None_right : forall {A} (xo : option A),
     either xo None = xo.
 Proof.
-Admitted.
+  intros A xo; destruct xo; reflexivity.
+Qed.
 
 (* [either] is associative, just like [++].
  *)
 Theorem either_assoc : forall {A} (xo yo zo : option A),
     either (either xo yo) zo = either xo (either yo zo).
 Proof.
-Admitted.
+  intros A xo yo zo; destruct xo, yo, zo; reflexivity.
+Qed.
 
 (* [head] should compute the head of a list, that is,
  * it should return [Some] with the first element of
  * the list if the list is nonempty, and [None]
  * if the list is empty.
  *)
-Fixpoint head {A} (xs : list A) : option A.
-Admitted.
+Fixpoint head {A} (xs : list A) : option A := match xs with
+  | nil => None
+  | a::_ => Some a
+  end.
 
 Example head_example : head [1; 2; 3] = Some 1.
 Proof.
-Admitted.
+  reflexivity.
+Qed.
 
 (* The following theorem makes a formal connection
  * between [either] and [++].
@@ -38,7 +43,8 @@ Admitted.
 Theorem either_app_head : forall {A} (xs ys : list A),
     head (xs ++ ys) = either (head xs) (head ys).
 Proof.
-Admitted.
+  destruct xs; reflexivity.
+Qed.
 
 (* [leftmost_Node] should compute the leftmost node of
  * a tree. 
@@ -47,23 +53,46 @@ Admitted.
  * recursion (i.e., pattern matching) on the [tree] argument,
  * without using the [flatten] operation.
  *)
-Fixpoint leftmost_Node {A} (t : tree A) : option A.
-Admitted.
+Fixpoint leftmost_Node {A} (t : tree A) : option A := match t with
+  | Leaf => None
+  | Node Leaf d _ => Some d
+  | Node l _ _ => leftmost_Node l
+  end.
 
 Example leftmost_Node_example :
     leftmost_Node (Node (Node Leaf 2 (Node Leaf 3 Leaf)) 1 Leaf)
     = Some 2.
 Proof.
-Admitted.
+  reflexivity.
+Qed.
 
 (* Prove that the leftmost node of the tree is the same
  * as the head of the list produced by flattening the tree
  * with an in-order traversal.
  *)
+Lemma flattened_node_has_element {A} : forall (l r: tree A) (d:A),
+    exists (v:A) (q:list A), flatten (Node l d r) = v::q.
+Proof.
+  intro l; elim l.
+  (* l=Leaf *)
+    intros r d; exists d, (flatten r); reflexivity.
+  (* l=Node ll lr ld *)
+    intros ll recl ld lr recr r d; elim (recl lr ld); clear recl.
+    intros v recl; elim recl; clear recl; intros q recl.
+    replace (flatten (Node (Node ll ld lr) d r)) with (flatten (Node ll ld lr)++d::flatten r) by reflexivity.
+    rewrite recl; exists v, (q ++ (d::(flatten r))); reflexivity.
+Qed.
 Theorem leftmost_Node_head : forall {A} (t : tree A),
       leftmost_Node t = head (flatten t).
 Proof.
-Admitted.
+  intros A t; elim t; clear t; [ reflexivity |].
+  intros l rec d r H; destruct l; [ reflexivity |].
+  replace (leftmost_Node (Node (Node l1 d0 l2) d r)) with (leftmost_Node (Node l1 d0 l2)) by reflexivity.
+  rewrite rec; clear rec.
+  replace (flatten (Node (Node l1 d0 l2) d r)) with (flatten (Node l1 d0 l2)++d::flatten r) by reflexivity.
+  elim (flattened_node_has_element l1 l2 d0); intros v tmp; elim tmp; clear tmp; intros q rep.
+  rewrite rep; reflexivity.
+Qed.
 
 (* Now let's work with the binary tries we defined earlier!
  *
@@ -75,18 +104,24 @@ Admitted.
  * for those keys that begin with [true], and the right subtree
  * contains entries for those keys that begin with [false].
  *)
-Fixpoint lookup {A} (k : list bool) (t : binary_trie A) : option A.
-Admitted.
+Fixpoint lookup {A} (k : list bool) (t : binary_trie A) : option A := match k, t with
+  | nil, Node _ d _ => d
+  | _, Leaf => None
+  | true::q, Node l _ _ => lookup q l
+  | false::q, Node _ _ r => lookup q r
+  end.
 
 Example lookup_example1 : lookup [] (Node Leaf (None : option nat) Leaf) = None.
 Proof.
-Admitted.
+  reflexivity.
+Qed.
 
 Example lookup_example2 : lookup [false; true]
     (Node (Node Leaf (Some 2) Leaf) None (Node (Node Leaf (Some 1) Leaf) (Some 3) Leaf))
                           = Some 1.
 Proof.
-Admitted.
+  reflexivity.
+Qed.
 
 (* [Leaf] represents an empty binary trie, so a lookup for
  * any key should return [None].
@@ -94,7 +129,8 @@ Admitted.
 Theorem lookup_empty {A} (k : list bool)
   : lookup k (Leaf : binary_trie A) = None.
 Proof.
-Admitted.
+  destruct k; [| destruct b ]; reflexivity.
+Qed.
 
 (* Define an operation to "insert" a key and optional value
  * into a binary trie. The [insert] definition should satisfy two
@@ -111,22 +147,32 @@ Admitted.
  * Hint: it may be helpful to define an auxiliary function that inserts
  * a key and optional value into the empty trie.
  *)
-Fixpoint insert {A} (k : list bool) (v : option A) (t : binary_trie A)
-  : binary_trie A.
-Admitted.
+Fixpoint insert {A} (k : list bool) (v : option A) (t : binary_trie A) : binary_trie A :=
+    match k, t with
+    | nil,Leaf => Node Leaf v Leaf
+    | nil, Node l _ r => Node l v r
+    | true::q, Leaf => Node (insert q v Leaf) None Leaf
+    | true::q, Node l d r => Node (insert q v l) d r
+    | false::q, Leaf => Node Leaf None (insert q v Leaf)
+    | false::q, Node l d r => Node l d (insert q v r)
+    end.
 
 Example insert_example1 : lookup [] (insert [] None (Node Leaf (Some 0) Leaf)) = None.
-Proof.
-Admitted.
+Proof eq_refl _.
 
 Example insert_example2 : lookup [] (insert [true] (Some 2) (Node Leaf (Some 0) Leaf)) = Some 0.
-Proof.
-Admitted.
+Proof eq_refl _.
 
-Theorem lookup_insert {A} (k : list bool) (v : option A) (t : binary_trie A)
-  : lookup k (insert k v t) = v.
+Theorem lookup_insert {A} : forall (k : list bool) (v : option A) (t : binary_trie A),
+    lookup k (insert k v t) = v.
 Proof.
-Admitted.
+  intro k; elim k; clear k; [ destruct t; reflexivity |]; intros a q rec v t.
+  destruct t.
+  (* Leaf *)
+    destruct a; exact (rec v Leaf).
+  (* Node t1 d t2 *)
+    destruct a; [ exact (rec v t1) | exact (rec v t2) ].
+Qed.
 
 
 (* You've reached the end of the problem set. Congrats!
@@ -142,10 +188,80 @@ Admitted.
  * can just leave everything below unmodified.
  *)
 
-Fixpoint left_biased_merge {A} (t t' : binary_trie A) : binary_trie A.
-Admitted.
+Fixpoint left_biased_merge {A} (t t' : binary_trie A) : binary_trie A :=
+  match (t, t') with
+    | (Leaf, Leaf) => Leaf
+    | (Node l d r, Leaf) => Node l d r
+    | (Leaf, Node l d r) => Node l d r
+    | (Node l d r, Node l' d' r') =>
+        Node (left_biased_merge l l') (either d d') (left_biased_merge r r')
+  end.
 
-Theorem lookup_left_biased_merge {A} (k : list bool) (t t' : binary_trie A)
-  : lookup k (left_biased_merge t t') = either (lookup k t) (lookup k t').
+Theorem lookup_left_biased_merge {A} (k : list bool)
+  : forall (t t' : binary_trie A),
+    lookup k (left_biased_merge t t') = either (lookup k t) (lookup k t').
 Proof.
-Admitted.
+  elim k.
+    (* nil *)
+    intros t t'.
+    case t.
+      (* Leaf *)
+      case t'.
+        reflexivity.
+        reflexivity.
+      (* Node l d r *)
+      intros l d r.
+      case t'.
+        (* Leaf *)
+        case d.
+          reflexivity.
+          reflexivity.
+        (* Node l' d' r' *)
+        intros l' d' r'.
+        case d, d'.
+          reflexivity.
+          reflexivity.
+          reflexivity.
+          reflexivity.
+    (* a::q *)
+    intros a q hyp1 t t'.
+    case t, t'.
+      (* Leaf, Leaf *)
+      case a.
+        reflexivity.
+        reflexivity.
+      (* Leaf, Node ... *)
+      case a, d.
+        reflexivity.
+        reflexivity.
+        reflexivity.
+        reflexivity.
+      (* Node ..., Leaf *)
+      assert (forall (x: option A), x = either x None) as subgoal.
+        intros x.
+        case x.
+          reflexivity.
+          reflexivity.
+      case a, d.
+        (* true, Some a *)
+        simpl.
+        exact (subgoal (lookup q t1)).
+        (* true, None *)
+        simpl.
+        exact (subgoal (lookup q t1)).
+        (* false, Some a *)
+        simpl.
+        exact (subgoal (lookup q t2)).
+        (* false, None *)
+        simpl.
+        exact (subgoal (lookup q t2)).
+      (* Node ..., Node ... *)
+      case a.
+        (* true *)
+        simpl.
+        exact (hyp1 t1 t'1).
+        (* false *)
+        simpl.
+        exact (hyp1 t2 t'2).
+Qed.
+
